Dafny/InsertionSortShuffle.dfy
@@ -1,0 +1,37 @@
+predicate Sorted(a:array<int>, low:int, high:int)
+	reads a
+{
+	0 <= low <= high <= a.Length &&
+	forall i,j :: low <= i < j < high ==> a[i] <= a[j]
+}
+
+method InsertionSortShuffle(a:array<int>)
+	modifies a
+	requires a.Length>1
+	ensures Sorted(a, 0, a.Length)
+	ensures multiset(a[..]) == multiset(old(a[..]))
+{
+	var curr := 1;
+	while (curr < a.Length)
+		invariant 1 <= curr <= a.Length
+		invariant Sorted(a, 0, curr);
+		invariant multiset(a[..]) == multiset(old(a[..]))
+	{
+		var num := a[curr];
+		var prev := curr - 1;
+		a[curr] := a[prev];
+
+		while (prev >= 0 && a[prev] > num)
+			invariant -1 <= prev < curr
+			invariant forall i :: prev < i < curr ==> a[i] >= num
+			invariant Sorted(a, 0, curr + 1)
+			invariant multiset(a[..]) + multiset([num]) - multiset([a[prev + 1]]) == multiset(old(a[..]))
+		{
+			a[prev + 1] := a[prev];
+			prev := prev - 1;
+		}
+
+		a[prev + 1] := num;
+		curr := curr + 1;
+	}
+}
